worked on asm level rewrites a bit

SSA/Projects/RISCV64/removeToIntToNat.lean
@@ -2,16 +2,16 @@ import SSA.Core.MLIRSyntax.EDSL
 set_option maxHeartbeats 1000000000000000000
 
 /-!
-  ## Dialect semantics
-  Every ISA instruction is modelled to operate on 64-bit bit vectors only.
-  This should allow to gain in automation using the bv_decide.
-
-  Additionally there is a rewrite of the function that defines the semantics in a pure BitVec operations
-  version avoiding toNat and toInt, which hinders proof automation by bv_decide. (at the moment only
-  for the instruction used in our lowering)
+  ## Dialect semantics bit-vectorization
+This file contains the `RV64` instruction semantics in a form that does not contain BitVec.toInt and BitVec.toNat.
+ToInt/ToNat calls hinder proof automation by bv_decide.
+To guarantee faithful rewrites of the dialect semantics as defined in Sail-Lean, this file also contains
+a proof for each rewrite.
+The instruction semantics suffixed by "bv" indicates that it is a transformed defintion where we removed
+toInt/toNat calls.
 -/
 
-/-  ## Additional introducded lemmas -/
+/-  ## Additional introducded lemmas on bit vectors -/
 namespace pure_semantics
 theorem sshiftRight_eq_sshiftRight_extractLsb {w : Nat}
     {lw : Nat} (hll : 2^lw = w) (hlw : lw > 0 )
@@ -28,13 +28,6 @@ theorem sshiftRight_eq_sshiftRight_extractLsb {w : Nat}
 
 theorem eq_of_toNat_eq3 {n} : ∀ {x y : BitVec n}, x.toNat = y.toNat → x = y
   | ⟨_, _⟩, ⟨_, _⟩, rfl => rfl
-  /-
-  proof strategy:
-  - show that if y has any set bits in indices [w..lw], then x.sshiftRight y = 0.
-    (If y is >= w, then x.sshiftRight y = 0)
-  - Otherwise, we know that y has no set bits in the range [w..lw], and therefore, y.toNat = y[0:lw].toNat
-    Hence, the shift amounts have the same value.
-  -/
 
 theorem sshiftRight_eq_setWidth_extractLsb_signExtend {w : Nat} (n : Nat) (x : BitVec w) :
     x.sshiftRight n =
@@ -44,7 +37,6 @@ theorem sshiftRight_eq_setWidth_extractLsb_signExtend {w : Nat} (n : Nat) (x : B
   simp [show i ≤ w - 1 by omega]
   simp [BitVec.getLsbD_signExtend]
   by_cases hni : (n + i) < w <;> simp [hni] <;> omega
-
 
 theorem BitVec.ofInt_toInt_eq_signExtend {w w' : Nat} {x : BitVec w} : BitVec.ofInt w' x.toInt = x.signExtend w' := by
   apply BitVec.eq_of_toInt_eq
@@ -61,7 +53,6 @@ theorem BitVec.ofInt_toInt_eq_signExtend {w w' : Nat} {x : BitVec w} : BitVec.of
       norm_cast
     rw [Int.bmod_eq_of_le_mul_two] <;> push_cast <;> omega
 
--- to do
 theorem toInt_toInt_ofInt_eq_toNat_toNat_ofNa{w w' : Nat }{x y : BitVec w } (h : w' ≤ w):
     BitVec.ofNat w' (x.toNat * y.toNat) = BitVec.ofInt w' (x.toInt * y.toInt) := by
   rw [BitVec.ofNat_mul]
@@ -72,17 +63,11 @@ theorem toInt_toInt_ofInt_eq_toNat_toNat_ofNa{w w' : Nat }{x y : BitVec w } (h :
   rw [BitVec.signExtend_eq_setWidth_of_le _ (by omega)]
   rw [BitVec.signExtend_eq_setWidth_of_le _ (by omega)]
 
-theorem toInt_ofInt_toNat_ofNat {w : Nat } {x : BitVec w} : BitVec.ofInt w (x.toInt) =  BitVec.ofNat w (x.toNat)
-  := by simp
-
-theorem toInt_toInt_eq_toInt (w : Nat) (x y : BitVec w) : BitVec.ofInt w (x.toInt *  y.toInt) = BitVec.ofInt w (x * y).toInt :=
-  by
-  simp only [BitVec.toInt_mul]
-  simp only [HMul.hMul, Mul.mul]
+theorem neg_ofNat_eq_ofInt_neg {w : Nat} (x : Nat) :
+    - BitVec.ofNat w x = BitVec.ofInt w (- x) := by
   apply BitVec.eq_of_toInt_eq
-  simp
+  simp [BitVec.toInt_neg, BitVec.toInt_ofNat]
 
-/-- An `extractLsb`' starting from `0` is the same as `setWidth`. -/
 @[simp]
 theorem extractLsb'_eq_setWidth {x : BitVec w} : x.extractLsb' 0 n = x.setWidth n := by
   ext i hi
@@ -99,8 +84,8 @@ theorem extractLsb'_ofInt_eq_ofInt {x : Int} {w w' : Nat}  {h : w ≤ w'} :
 
 theorem extractLsb'_ofInt_eq_ofInt_ofNat {x : Nat} {w w' : Nat}  {h : w ≤ w'} :
     (BitVec.extractLsb' 0 w (BitVec.ofInt w' x)) = (BitVec.ofInt w x) := by
-      apply extractLsb'_ofInt_eq_ofInt
-      exact h
+  apply extractLsb'_ofInt_eq_ofInt
+  exact h
 
 theorem BitVec.setWidth_signExtend_eq_self {w w' : Nat} {x : BitVec w} (h : w ≤ w') : (x.signExtend w').setWidth w = x := by
   ext i hi
@@ -108,49 +93,46 @@ theorem BitVec.setWidth_signExtend_eq_self {w w' : Nat} {x : BitVec w} (h : w �
   omega
 
 
-def ADDIW_pure64 (imm : BitVec 12) (rs1_val : BitVec 64) :  BitVec 64 :=
+def ADDIW_pure64 (imm : BitVec 12) (rs1_val : BitVec 64) : BitVec 64 :=
      BitVec.signExtend 64 (BitVec.setWidth 32 (BitVec.add (BitVec.signExtend 64 imm) rs1_val))
 
 def UTYPE_pure64_lui (imm : BitVec 20) (pc : BitVec 64) : BitVec 64 :=
-     BitVec.signExtend 64 (imm ++ (0x000 : (BitVec 12)))
+  BitVec.signExtend 64 (imm ++ (0x000 : (BitVec 12)))
 
-def UTYPE_pure64_AUIPC (imm : BitVec 20) (pc : BitVec 64)  : BitVec 64 :=
-    BitVec.add (BitVec.signExtend 64 (BitVec.append imm (0x000 : (BitVec 12)))) pc
+def UTYPE_pure64_AUIPC (imm : BitVec 20) (pc : BitVec 64) : BitVec 64 :=
+  BitVec.add (BitVec.signExtend 64 (BitVec.append imm (0x000 : (BitVec 12)))) pc
 
 def SHIFTIWOP_pure64_RISCV_SLLIW (shamt : BitVec 5) (rs1_val : BitVec 64) : BitVec 64 :=
-    BitVec.signExtend 64 (BitVec.shiftLeft (BitVec.extractLsb' 0 32 rs1_val) (shamt).toNat)
+  BitVec.signExtend 64 (BitVec.shiftLeft (BitVec.extractLsb' 0 32 rs1_val) (shamt).toNat)
 
 def SHIFTIWOP_pure64_RISCV_SLLIW_bv (shamt : BitVec 5) (rs1_val : BitVec 64) : BitVec 64 :=
-    BitVec.signExtend 64 ( (BitVec.extractLsb' 0 32 rs1_val)  <<< (shamt))
+  BitVec.signExtend 64 ( (BitVec.extractLsb' 0 32 rs1_val)  <<< (shamt))
 
 theorem SHIFTIWOP_pure64_RISCV_SLLIW_eq_SHIFTIWOP_pure64_RISCV_SLLIW_bv (shamt : BitVec 5) (rs1_val : BitVec 64) :
   SHIFTIWOP_pure64_RISCV_SLLIW (shamt ) (rs1_val ) = SHIFTIWOP_pure64_RISCV_SLLIW_bv (shamt) (rs1_val) :=
-    by
-    unfold SHIFTIWOP_pure64_RISCV_SLLIW SHIFTIWOP_pure64_RISCV_SLLIW_bv
-    rfl
+  by
+  unfold SHIFTIWOP_pure64_RISCV_SLLIW SHIFTIWOP_pure64_RISCV_SLLIW_bv
+  rfl
 
 def SHIFTIWOP_pure64_RISCV_SRLIW (shamt : BitVec 5) (rs1_val : BitVec 64) : BitVec 64 :=
-    BitVec.signExtend 64 (BitVec.ushiftRight (BitVec.extractLsb' 0 32 rs1_val) (shamt).toNat)
+  BitVec.signExtend 64 (BitVec.ushiftRight (BitVec.extractLsb' 0 32 rs1_val) (shamt).toNat)
 
 def SHIFTIWOP_pure64_RISCV_SRLIW_bv (shamt : BitVec 5) (rs1_val : BitVec 64) : BitVec 64 :=
-    BitVec.signExtend 64 ( (BitVec.extractLsb' 0 32 rs1_val) >>> (shamt))
+  BitVec.signExtend 64 ( (BitVec.extractLsb' 0 32 rs1_val) >>> (shamt))
 
 theorem  SHIFTIWOP_pure64_RISCV_SRLIW_eq_SHIFTIWOP_pure64_RISCV_SRLIW_bv (shamt : BitVec 5) (rs1_val : BitVec 64) :
-    SHIFTIWOP_pure64_RISCV_SRLIW (shamt) (rs1_val) =  SHIFTIWOP_pure64_RISCV_SRLIW_bv (shamt) (rs1_val) :=
-    by
-    unfold SHIFTIWOP_pure64_RISCV_SRLIW SHIFTIWOP_pure64_RISCV_SRLIW_bv
-    rfl
+  SHIFTIWOP_pure64_RISCV_SRLIW (shamt) (rs1_val) =  SHIFTIWOP_pure64_RISCV_SRLIW_bv (shamt) (rs1_val) :=
+  by
+  unfold SHIFTIWOP_pure64_RISCV_SRLIW SHIFTIWOP_pure64_RISCV_SRLIW_bv
+  rfl
 
-def SHIFTIWOP_pure64_RISCV_SRAIW (shamt : BitVec 5) (rs1_val : BitVec 64) : BitVec 64
-    :=
+def SHIFTIWOP_pure64_RISCV_SRAIW (shamt : BitVec 5) (rs1_val : BitVec 64) : BitVec 64 :=
     BitVec.signExtend 64
       (BitVec.setWidth 32
        (BitVec.extractLsb
          (31 + shamt.toNat)
           shamt.toNat
-          (BitVec.signExtend ((32) + shamt.toNat) (BitVec.extractLsb 31 0 rs1_val))
-        )
-      )
+          (BitVec.signExtend ((32) + shamt.toNat) (BitVec.extractLsb 31 0 rs1_val))))
 
 def SHIFTIWOP_pure64_RISCV_SRAIW_bv (shamt : BitVec 5) (rs1_val : BitVec 64) : BitVec 64 :=
   BitVec.signExtend 64 (BitVec.sshiftRight' (BitVec.extractLsb 31 0 rs1_val) shamt)
@@ -162,65 +144,64 @@ theorem SHIFTIWOP_pure64_RISCV_SRAIW_eq_SHIFTIWOP_pure64_RISCV_SRAIW_bv (shamt :
   rw [← sshiftRight_eq_setWidth_extractLsb_signExtend]
   rfl
 
-def SHIFTIOP_pure64_RISCV_SLLI (shamt : BitVec 6) (rs1_val : BitVec 64)  : BitVec 64
-    := BitVec.shiftLeft rs1_val shamt.toNat
+def SHIFTIOP_pure64_RISCV_SLLI (shamt : BitVec 6) (rs1_val : BitVec 64) : BitVec 64 :=
+  BitVec.shiftLeft rs1_val shamt.toNat
 
-def  SHIFTIOP_pure64_RISCV_SLLI_bv (shamt : BitVec 6) (rs1_val : BitVec 64)  : BitVec 64 :=
+def  SHIFTIOP_pure64_RISCV_SLLI_bv (shamt : BitVec 6) (rs1_val : BitVec 64) : BitVec 64 :=
   rs1_val <<< shamt
 
-
 theorem SHIFTIOP_pure64_RISCV_SLLI_eq_SHIFTIOP_pure64_RISCV_SLLI_bv :
-    SHIFTIOP_pure64_RISCV_SLLI (shamt) (rs1_val) = SHIFTIOP_pure64_RISCV_SLLI_bv (shamt) (rs1_val) := by
+  SHIFTIOP_pure64_RISCV_SLLI (shamt) (rs1_val) = SHIFTIOP_pure64_RISCV_SLLI_bv (shamt) (rs1_val) := by
   unfold SHIFTIOP_pure64_RISCV_SLLI SHIFTIOP_pure64_RISCV_SLLI_bv
   simp
 
 def SHIFTIOP_pure64_RISCV_SRLI (shamt : BitVec 6) (rs1_val : BitVec 64) : BitVec 64 :=
-    BitVec.ushiftRight rs1_val shamt.toNat
+  BitVec.ushiftRight rs1_val shamt.toNat
 
 def SHIFTIOP_pure64_RISCV_SRLI_bv (shamt : BitVec 6) (rs1_val : BitVec 64) : BitVec 64 :=
-     rs1_val >>> shamt
+  rs1_val >>> shamt
 
 theorem SHIFTIOP_pure64_RISCV_SRLI_eq_SHIFTIOP_pure64_RISCV_SRLI_bv (shamt : BitVec 6) (rs1_val : BitVec 64) :
-    SHIFTIOP_pure64_RISCV_SRLI (shamt) (rs1_val) = SHIFTIOP_pure64_RISCV_SRLI_bv (shamt) (rs1_val) := by
+  SHIFTIOP_pure64_RISCV_SRLI (shamt) (rs1_val) = SHIFTIOP_pure64_RISCV_SRLI_bv (shamt) (rs1_val) := by
   unfold SHIFTIOP_pure64_RISCV_SRLI SHIFTIOP_pure64_RISCV_SRLI_bv
   simp
 
-def SHIFTIOP_pure64_RISCV_SRAI (shamt : (BitVec 6)) (rs1_val : (BitVec 64)): BitVec 64 :=
-    let value := rs1_val ;
-    let shift := shamt.toNat;
-    BitVec.setWidth 64 (BitVec.extractLsb (63 + shift) shift (BitVec.signExtend (64 + shift) value))
+def SHIFTIOP_pure64_RISCV_SRAI (shamt : BitVec 6) (rs1_val : BitVec 64): BitVec 64 :=
+  let value := rs1_val ;
+  let shift := shamt.toNat;
+  BitVec.setWidth 64 (BitVec.extractLsb (63 + shift) shift (BitVec.signExtend (64 + shift) value))
 
-def SHIFTIOP_pure64_RISCV_SRAI_bv (shamt : (BitVec 6)) (rs1_val : (BitVec 64)): BitVec 64 :=
-    BitVec.sshiftRight' rs1_val  shamt
+def SHIFTIOP_pure64_RISCV_SRAI_bv (shamt : BitVec 6) (rs1_val : BitVec 64): BitVec 64 :=
+  BitVec.sshiftRight' rs1_val  shamt
 
-theorem SHIFTIOP_pure64_RISCV_SRAI_eq_SHIFTIOP_pure64_RISCV_SRAI_bv (shamt : (BitVec 6)) (rs1_val : (BitVec 64)) :
+theorem SHIFTIOP_pure64_RISCV_SRAI_eq_SHIFTIOP_pure64_RISCV_SRAI_bv (shamt : BitVec 6) (rs1_val : BitVec 64) :
   SHIFTIOP_pure64_RISCV_SRAI (shamt) (rs1_val ) = SHIFTIOP_pure64_RISCV_SRAI_bv (shamt) (rs1_val ) :=
   by
   unfold SHIFTIOP_pure64_RISCV_SRAI SHIFTIOP_pure64_RISCV_SRAI_bv
   simp
-  rw [sshiftRight_eq_setWidth_extractLsb_signExtend] -- own lemma
+  rw [sshiftRight_eq_setWidth_extractLsb_signExtend]
 
 def RTYPEW_pure64_RISCV_ADDW (rs2_val : BitVec 64) (rs1_val : BitVec 64) : BitVec 64 :=
-      let rs1_val32 := BitVec.extractLsb' 0 32 rs1_val;
-      let rs2_val32 := BitVec.extractLsb' 0 32 rs2_val;
-      BitVec.signExtend 64 (BitVec.add rs1_val32 rs2_val32)
+  let rs1_val32 := BitVec.extractLsb' 0 32 rs1_val;
+  let rs2_val32 := BitVec.extractLsb' 0 32 rs2_val;
+  BitVec.signExtend 64 (BitVec.add rs1_val32 rs2_val32)
 
 def RTYPEW_pure64_RISCV_SUBW (rs2_val : BitVec 64) (rs1_val : BitVec 64) : BitVec 64 :=
-      let rs1_val32 := BitVec.extractLsb' 0 32 rs1_val;
-      let rs2_val32 := BitVec.extractLsb' 0 32 rs2_val;
-      BitVec.signExtend 64 (BitVec.sub rs1_val32 rs2_val32)
+  let rs1_val32 := BitVec.extractLsb' 0 32 rs1_val;
+  let rs2_val32 := BitVec.extractLsb' 0 32 rs2_val;
+  BitVec.signExtend 64 (BitVec.sub rs1_val32 rs2_val32)
 
 def RTYPEW_pure64_RISCV_SLLW (rs2_val : BitVec 64) (rs1_val : BitVec 64) : BitVec 64 :=
-    let rs1_val32 := BitVec.extractLsb' 0 32 rs1_val;
-    let rs2_val32 := BitVec.extractLsb' 0 32 rs2_val;
-    let shamt := BitVec.extractLsb' 0 5 rs2_val32;
-    BitVec.signExtend 64 (BitVec.shiftLeft rs1_val32 shamt.toNat)
+  let rs1_val32 := BitVec.extractLsb' 0 32 rs1_val;
+  let rs2_val32 := BitVec.extractLsb' 0 32 rs2_val;
+  let shamt := BitVec.extractLsb' 0 5 rs2_val32;
+  BitVec.signExtend 64 (BitVec.shiftLeft rs1_val32 shamt.toNat)
 
 def RTYPEW_pure64_RISCV_SLLW_bv (rs2_val : BitVec 64) (rs1_val : BitVec 64) : BitVec 64 :=
-    let rs1_val32 := BitVec.extractLsb' 0 32 rs1_val;
-    let rs2_val32 := BitVec.extractLsb' 0 32 rs2_val;
-    let shamt := BitVec.extractLsb' 0 5 rs2_val32;
-    BitVec.signExtend 64 (rs1_val32 <<< shamt)
+  let rs1_val32 := BitVec.extractLsb' 0 32 rs1_val;
+  let rs2_val32 := BitVec.extractLsb' 0 32 rs2_val;
+  let shamt := BitVec.extractLsb' 0 5 rs2_val32;
+  BitVec.signExtend 64 (rs1_val32 <<< shamt)
 
 theorem  RTYPEW_pure64_RISCV_SLLW_eq_RTYPEW_pure64_RISCV_SLLW_bv (rs2_val : BitVec 64) (rs1_val : BitVec 64) :
   RTYPEW_pure64_RISCV_SLLW (rs2_val) (rs1_val) =  RTYPEW_pure64_RISCV_SLLW_bv (rs2_val) (rs1_val) :=
@@ -229,26 +210,25 @@ theorem  RTYPEW_pure64_RISCV_SLLW_eq_RTYPEW_pure64_RISCV_SLLW_bv (rs2_val : BitV
   simp only [extractLsb'_eq_setWidth, Nat.reduceLeDiff, BitVec.setWidth_setWidth_of_le,
     BitVec.toNat_setWidth, Nat.reducePow, BitVec.shiftLeft_eq, BitVec.shiftLeft_eq']
 
+def RTYPEW_pure64_RISCV_SRLW (rs2_val : BitVec 64) (rs1_val : BitVec 64) : BitVec 64 :=
+  let rs1_val32 := BitVec.extractLsb' 0 32 rs1_val;
+  let rs2_val32 := BitVec.extractLsb' 0 32 rs2_val;
+  let shamt := BitVec.extractLsb' 0 5 rs2_val32;
+  BitVec.signExtend 64 (BitVec.ushiftRight rs1_val32 shamt.toNat)
 
-def RTYPEW_pure64_RISCV_SRLW (rs2_val : BitVec 64) (rs1_val : BitVec 64)  : BitVec 64 :=
-    let rs1_val32 := BitVec.extractLsb' 0 32 rs1_val;
-    let rs2_val32 := BitVec.extractLsb' 0 32 rs2_val;
-    let shamt := BitVec.extractLsb' 0 5 rs2_val32;
-    BitVec.signExtend 64 (BitVec.ushiftRight rs1_val32 shamt.toNat)
-
-def RTYPEW_pure64_RISCV_SRLW_bv (rs2_val : BitVec 64) (rs1_val : BitVec 64)  : BitVec 64 :=
-    let rs1_val32 := BitVec.extractLsb' 0 32 rs1_val;
-    let rs2_val32 := BitVec.extractLsb' 0 32 rs2_val;
-    let shamt := BitVec.extractLsb' 0 5 rs2_val32;
-    BitVec.signExtend 64 (rs1_val32 >>> shamt)
+def RTYPEW_pure64_RISCV_SRLW_bv (rs2_val : BitVec 64) (rs1_val : BitVec 64) : BitVec 64 :=
+  let rs1_val32 := BitVec.extractLsb' 0 32 rs1_val;
+  let rs2_val32 := BitVec.extractLsb' 0 32 rs2_val;
+  let shamt := BitVec.extractLsb' 0 5 rs2_val32;
+  BitVec.signExtend 64 (rs1_val32 >>> shamt)
 
 theorem RTYPEW_pure64_RISCV_SLLW_eq_RTYPEW_pure64_RISCV_SRLW_bv (rs2_val : BitVec 64) (rs1_val : BitVec 64) :
-    RTYPEW_pure64_RISCV_SRLW (rs2_val) (rs1_val) =  RTYPEW_pure64_RISCV_SRLW_bv (rs2_val) (rs1_val) := by
+  RTYPEW_pure64_RISCV_SRLW (rs2_val) (rs1_val) =  RTYPEW_pure64_RISCV_SRLW_bv (rs2_val) (rs1_val) := by
   unfold RTYPEW_pure64_RISCV_SRLW RTYPEW_pure64_RISCV_SRLW_bv
   simp
 
-def RTYPEW_pure64_RISCV_SRAW (rs2_val : (BitVec 64)) (rs1_val : (BitVec 64)) :=
-BitVec.signExtend 64
+def RTYPEW_pure64_RISCV_SRAW (rs2_val : BitVec 64) (rs1_val : BitVec 64) :=
+  BitVec.signExtend 64
            (BitVec.setWidth 32
               (BitVec.extractLsb
                  (31 + rs2_val.toNat % 4294967296 % 32)
@@ -256,70 +236,69 @@ BitVec.signExtend 64
                           (BitVec.signExtend (32 + rs2_val.toNat % 4294967296 % 32)
                               (BitVec.extractLsb 31 0 rs1_val))))
 
-def RTYPEW_pure64_RISCV_SRAW_bv (rs2_val : (BitVec 64)) (rs1_val : (BitVec 64)) :=
-BitVec.signExtend 64
-      (BitVec.sshiftRight' (BitVec.extractLsb 31 0 rs1_val)  (BitVec.extractLsb 4 0 rs2_val))
+def RTYPEW_pure64_RISCV_SRAW_bv (rs2_val : BitVec 64) (rs1_val : BitVec 64) :=
+  BitVec.signExtend 64
+  (BitVec.sshiftRight' (BitVec.extractLsb 31 0 rs1_val)  (BitVec.extractLsb 4 0 rs2_val))
 
-
-theorem RTYPEW_pure64_RISCV_SRAW_eq_RTYPEW_pure64_RISCV_SRAW_bv (rs2_val : (BitVec 64)) (rs1_val : (BitVec 64))  :
+theorem RTYPEW_pure64_RISCV_SRAW_eq_RTYPEW_pure64_RISCV_SRAW_bv (rs2_val : BitVec 64) (rs1_val : BitVec 64) :
   RTYPEW_pure64_RISCV_SRAW (rs2_val) (rs1_val) = RTYPEW_pure64_RISCV_SRAW_bv (rs2_val) (rs1_val) :=
-   by
-   unfold RTYPEW_pure64_RISCV_SRAW RTYPEW_pure64_RISCV_SRAW_bv
-   rw [← sshiftRight_eq_setWidth_extractLsb_signExtend]
-   simp
+  by
+  unfold RTYPEW_pure64_RISCV_SRAW RTYPEW_pure64_RISCV_SRAW_bv
+  rw [← sshiftRight_eq_setWidth_extractLsb_signExtend]
+  simp
 
-def RTYPE_pure64_RISCV_ADD (rs2_val : BitVec 64) (rs1_val : BitVec 64) :BitVec 64 :=
-      BitVec.add rs1_val rs2_val
+def RTYPE_pure64_RISCV_ADD (rs2_val : BitVec 64) (rs1_val : BitVec 64) : BitVec 64 :=
+  BitVec.add rs1_val rs2_val
 
 def RTYPE_pure64_RISCV_SLT (rs2_val : BitVec 64) (rs1_val : BitVec 64) : BitVec 64 :=
-    let b := BitVec.slt rs1_val rs2_val;
-    BitVec.setWidth 64 (BitVec.ofBool b)
+  let b := BitVec.slt rs1_val rs2_val;
+  BitVec.setWidth 64 (BitVec.ofBool b)
 
 def RTYPE_pure64_RISCV_SLTU (rs2_val : BitVec 64) (rs1_val : BitVec 64) : BitVec 64 :=
-    let b := BitVec.ult rs1_val rs2_val;
-      BitVec.setWidth 64 (BitVec.ofBool b)
+  let b := BitVec.ult rs1_val rs2_val;
+  BitVec.setWidth 64 (BitVec.ofBool b)
 
 def RTYPE_pure64_RISCV_AND (rs2_val : BitVec 64) (rs1_val : BitVec 64) : BitVec 64 :=
-      BitVec.and rs2_val rs1_val
+  BitVec.and rs2_val rs1_val
 
 def RTYPE_pure64_RISCV_OR(rs2_val : BitVec 64) (rs1_val : BitVec 64) : BitVec 64 :=
-      BitVec.or rs2_val rs1_val
+  BitVec.or rs2_val rs1_val
 
 def RTYPE_pure64_RISCV_XOR(rs2_val : BitVec 64) (rs1_val : BitVec 64) : BitVec 64 :=
-      BitVec.xor rs2_val rs1_val
+  BitVec.xor rs2_val rs1_val
 
 def RTYPE_pure64_RISCV_SLL (rs2_val : BitVec 64) (rs1_val : BitVec 64) : BitVec 64 :=
-       let shamt := (BitVec.extractLsb 5 0 rs2_val).toNat;
-       BitVec.shiftLeft rs1_val shamt
+  let shamt := (BitVec.extractLsb 5 0 rs2_val).toNat;
+  BitVec.shiftLeft rs1_val shamt
 
 def RTYPE_pure64_RISCV_SLL_bv (rs2_val : BitVec 64) (rs1_val : BitVec 64) : BitVec 64 :=
-       let shamt := (BitVec.extractLsb 5 0 rs2_val);
-       rs1_val <<< shamt
+  let shamt := (BitVec.extractLsb 5 0 rs2_val);
+  rs1_val <<< shamt
 
 theorem RTYPE_pure64_RISCV_SLL_eq_RTYPE_pure64_RISCV_SLL_bv  (rs2_val : BitVec 64) (rs1_val : BitVec 64) :
-    RTYPE_pure64_RISCV_SLL = RTYPE_pure64_RISCV_SLL_bv := by
+  RTYPE_pure64_RISCV_SLL (rs2_val) (rs1_val)= RTYPE_pure64_RISCV_SLL_bv (rs2_val) (rs1_val) := by
   unfold RTYPE_pure64_RISCV_SLL  RTYPE_pure64_RISCV_SLL_bv
   simp
 
 def RTYPE_pure64_RISCV_SRL (rs2_val : BitVec 64) (rs1_val : BitVec 64) : BitVec 64 :=
-      let shamt := (BitVec.extractLsb 5 0 rs2_val).toNat;
-      BitVec.ushiftRight rs1_val shamt
+  let shamt := (BitVec.extractLsb 5 0 rs2_val).toNat;
+  BitVec.ushiftRight rs1_val shamt
 
 def RTYPE_pure64_RISCV_SRL_bv (rs2_val : BitVec 64) (rs1_val : BitVec 64) : BitVec 64 :=
-      let shamt := (BitVec.extractLsb 5 0 rs2_val)
-      rs1_val  >>> shamt
+  let shamt := (BitVec.extractLsb 5 0 rs2_val)
+  rs1_val >>> shamt
 
 theorem RTYPE_pure64_RISCV_SRL_eq_RTYPE_pure64_RISCV_SRL_bv  (rs2_val : BitVec 64) (rs1_val : BitVec 64) :
-  RTYPE_pure64_RISCV_SRL = RTYPE_pure64_RISCV_SRL_bv :=
+  RTYPE_pure64_RISCV_SRL (rs2_val) (rs1_val) = RTYPE_pure64_RISCV_SRL_bv (rs2_val) (rs1_val) :=
   by
   unfold RTYPE_pure64_RISCV_SRL RTYPE_pure64_RISCV_SRL_bv
   simp
 
 def RTYPE_pure64_RISCV_SUB (rs2_val : BitVec 64) (rs1_val : BitVec 64) : BitVec 64 :=
-    BitVec.sub rs1_val rs2_val
+  BitVec.sub rs1_val rs2_val
 
 def RTYPE_pure64_RISCV_SRA (rs2_val : BitVec 64) (rs1_val : BitVec 64) :=
-BitVec.setWidth 64
+  BitVec.setWidth 64
       (BitVec.extractLsb
         (63 + (BitVec.extractLsb 5 0 rs2_val).toNat)
         (BitVec.extractLsb 5 0 rs2_val).toNat
@@ -327,10 +306,10 @@ BitVec.setWidth 64
           (64 + (BitVec.extractLsb 5 0 rs2_val).toNat) rs1_val))
 
 def RTYPE_pure64_RISCV_SRA_bv (rs2_val : BitVec 64) (rs1_val : BitVec 64) : BitVec 64 :=
-  BitVec.sshiftRight' rs1_val  (BitVec.extractLsb 5 0 rs2_val)
+  BitVec.sshiftRight' rs1_val (BitVec.extractLsb 5 0 rs2_val)
 
 theorem RTYPE_pure64_RISCV_SRA_eqRTYPE_pure64_RISCV_SRA_bv (rs2_val : BitVec 64) (rs1_val : BitVec 64) :
-  RTYPE_pure64_RISCV_SRA  (rs2_val) (rs1_val) = RTYPE_pure64_RISCV_SRA_bv  (rs2_val) (rs1_val ) := by
+  RTYPE_pure64_RISCV_SRA  (rs2_val) (rs1_val) = RTYPE_pure64_RISCV_SRA_bv (rs2_val) (rs1_val) := by
   unfold RTYPE_pure64_RISCV_SRA RTYPE_pure64_RISCV_SRA_bv
   rw [BitVec.sshiftRight']
   rw [sshiftRight_eq_setWidth_extractLsb_signExtend]
@@ -346,7 +325,6 @@ def REMW_pure64_unsigned_bv (rs2_val : (BitVec 64)) (rs1_val : (BitVec 64)) : Bi
   BitVec.signExtend 64
       ((BitVec.extractLsb 31 0 rs1_val).umod (BitVec.extractLsb 31 0 rs2_val))
 
--- to do !!!!!!
 theorem REMW_pure64_unsigned_eq_REMW_pure64_unsigned_bv (rs2_val : BitVec 64) (rs1_val : BitVec 64) :
   REMW_pure64_unsigned (rs2_val : BitVec 64) (rs1_val : BitVec 64) =  REMW_pure64_unsigned_bv (rs2_val : (BitVec 64)) (rs1_val : (BitVec 64)) :=
   by
@@ -364,7 +342,7 @@ theorem REMW_pure64_unsigned_eq_REMW_pure64_unsigned_bv (rs2_val : BitVec 64) (r
       obtain h : (BitVec.extractLsb' 0 32 rs2_val) = 0#_ :=
         BitVec.eq_of_toNat_eq ht
       obtain h1 : (0#32).toNat = 0 := by bv_decide
-      simp only [BitVec.toNat_setWidth, Int.ofNat_emod, Int.natCast_pow, Nat.cast_ofNat,
+      simp only [BitVec.toNat_setWidth, Int.natCast_emod, Int.natCast_pow, Nat.cast_ofNat,
         BitVec.umod_eq]
       rw [show 0 = (0#32).toNat by omega, ← BitVec.toNat_eq] at ht
       conv at ht =>
@@ -381,7 +359,7 @@ theorem REMW_pure64_unsigned_eq_REMW_pure64_unsigned_bv (rs2_val : BitVec 64) (r
   case isFalse hf =>
       congr
       simp only [Nat.sub_zero, Nat.reduceAdd, BitVec.extractLsb_toNat, Nat.shiftRight_zero,
-        Nat.reducePow, Int.ofNat_emod, Nat.cast_ofNat, BitVec.umod_eq]
+        Nat.reducePow, Int.natCast_emod, Nat.cast_ofNat, BitVec.umod_eq]
       simp at hf
       apply BitVec.eq_of_toInt_eq
       simp only [BitVec.toInt_ofInt, Nat.reducePow, BitVec.toInt_umod, BitVec.extractLsb_toNat,
@@ -400,7 +378,7 @@ def REMW_pure64_signed_bv (rs2_val : (BitVec 64)) (rs1_val : (BitVec 64)) : BitV
       ((BitVec.extractLsb 31 0 rs1_val).srem (BitVec.extractLsb 31 0 rs2_val))
 
 theorem REMW_pure64_signed_eq_REMW_pure64_signed  (rs2_val : BitVec 64) (rs1_val : BitVec 64) :
- REMW_pure64_signed (rs2_val) (rs1_val) = REMW_pure64_signed_bv (rs2_val) (rs1_val) :=
+   REMW_pure64_signed (rs2_val) (rs1_val) = REMW_pure64_signed_bv (rs2_val) (rs1_val) :=
     by
     unfold REMW_pure64_signed REMW_pure64_signed_bv
     rw [extractLsb'_ofInt_eq_ofInt (h:= by simp )]
@@ -424,7 +402,10 @@ def REM_pure64_unsigned (rs2_val : BitVec 64) (rs1_val : BitVec 64) : BitVec 64 
 def REM_pure64_unsigned_bv (rs2_val : BitVec 64) (rs1_val : BitVec 64) : BitVec 64  :=
    (if (rs2_val) = 0 then (rs1_val)  else ((rs1_val).umod (rs2_val)))
 
--- proof in process.
+/- proof in process. The following lemma does not yet exist in Lean's bit vector library.
+We are confident that this holds and the lemma is in process of being proven and
+added to the bit vector library.
+-/
 theorem toInt_smod {x y : BitVec w} :
     (x.smod y).toInt = x.toInt.fmod y.toInt := by sorry
 
@@ -433,19 +414,20 @@ theorem  REM_pure64_unsigned_eq_REM_pure64_unsigned_bv (rs2_val : BitVec 64) (rs
   unfold REM_pure64_unsigned REM_pure64_unsigned_bv
   rw [extractLsb'_ofInt_eq_ofInt (h:= by simp )]
   split
-  · case isTrue isZero =>
+  case isTrue isZero =>
       simp only [Int.natCast_eq_zero] at isZero
       obtain rfl : rs2_val = 0#_ :=
         BitVec.eq_of_toNat_eq isZero
       simp
-  · case isFalse nonZero =>
+  case isFalse nonZero =>
       simp only [Int.natCast_eq_zero] at nonZero
       simp only [BitVec.ofNat_eq_ofNat, BitVec.umod_eq]
       have h:= (BitVec.toNat_ne_iff_ne (x:=rs2_val) (y:= 0)).mp nonZero
       have h2:= (BitVec.toNat_ne_iff_ne (x:=rs2_val) (y:= 0)).mpr h
       split
-      · contradiction
-      · apply BitVec.eq_of_toInt_eq
+      case isTrue => contradiction
+      case isFalse =>
+        apply BitVec.eq_of_toInt_eq
         simp only [BitVec.toInt_ofInt, Nat.reducePow, BitVec.toInt_umod]
         rfl
 
@@ -456,7 +438,7 @@ def REM_pure64_signed (rs2_val : BitVec 64) (rs1_val : BitVec 64) : BitVec 64  :
 def REM_pure64_signed_bv (rs2_val : BitVec 64) (rs1_val : BitVec 64) : BitVec 64 :=
    rs1_val.srem rs2_val
 
-theorem  REM_pure64_signed_eq_REM_pure64_signed_bv (rs2_val : BitVec 64) (rs1_val : BitVec 64) :
+theorem REM_pure64_signed_eq_REM_pure64_signed_bv (rs2_val : BitVec 64) (rs1_val : BitVec 64) :
     REM_pure64_signed (rs2_val) (rs1_val) = REM_pure64_signed_bv (rs2_val) (rs1_val) := by
   unfold REM_pure64_signed REM_pure64_signed_bv
   rw [extractLsb'_ofInt_eq_ofInt (h:= by simp)]
@@ -470,17 +452,17 @@ theorem  REM_pure64_signed_eq_REM_pure64_signed_bv (rs2_val : BitVec 64) (rs1_va
     rw [← BitVec.toInt_srem ]
     rw [BitVec.ofInt_toInt]
 
-def MULW_pure64 (rs2_val : (BitVec 64)) (rs1_val : (BitVec 64)) : BitVec 64 :=
+def MULW_pure64 (rs2_val : BitVec 64) (rs1_val :BitVec 64) : BitVec 64 :=
   BitVec.signExtend 64
     (BitVec.extractLsb 31 0
       (BitVec.extractLsb' 0 64
         (BitVec.ofInt 65 ((BitVec.extractLsb 31 0 rs1_val).toInt * (BitVec.extractLsb 31 0 rs2_val).toInt))))
 
-def MULW_pure64_bv (rs2_val : (BitVec 64)) (rs1_val : (BitVec 64)) : BitVec 64 :=
+def MULW_pure64_bv (rs2_val : BitVec 64) (rs1_val : BitVec 64) : BitVec 64 :=
   BitVec.signExtend 64
     (((BitVec.extractLsb 31 0 rs1_val) * (BitVec.extractLsb 31 0 rs2_val)))
 
-theorem MULW_pure64_eq_MULW_pure64_bv (rs2_val : (BitVec 64)) (rs1_val : (BitVec 64))  :
+theorem MULW_pure64_eq_MULW_pure64_bv (rs2_val : BitVec 64) (rs1_val : BitVec 64)  :
   MULW_pure64 (rs2_val) (rs1_val) = MULW_pure64_bv  (rs2_val) (rs1_val) :=
     by
     unfold MULW_pure64 MULW_pure64_bv
@@ -493,19 +475,13 @@ theorem MULW_pure64_eq_MULW_pure64_bv (rs2_val : (BitVec 64)) (rs1_val : (BitVec
     simp only [BitVec.toInt_extractLsb, Nat.shiftRight_zero, Nat.sub_zero, Nat.reduceAdd,
       Nat.reducePow, BitVec.toInt_ofInt, Int.mul_bmod_bmod, Int.bmod_mul_bmod, BitVec.toInt_mul]
 
-/-!
-## mul operations flags
- the suffix indicates how the flags are assumed to be set.
-{ high := _, signed_rs1:= _, signed_rs2 := _  }
--/
 def MUL_pure64_fff (rs2_val : BitVec 64) (rs1_val : BitVec 64) : BitVec 64 :=
      BitVec.extractLsb 63 0 (BitVec.extractLsb' 0 128 (BitVec.ofInt 129 (rs1_val.toNat * rs2_val.toNat)))
 
-def  MUL_pure64_fff_bv (rs2_val : BitVec 64) (rs1_val : BitVec 64) : BitVec 64 :=  rs2_val * rs1_val
+def MUL_pure64_fff_bv (rs2_val : BitVec 64) (rs1_val : BitVec 64) : BitVec 64 :=  rs2_val * rs1_val
 
-theorem mul_eq_mul_pretty (rs2_val : BitVec 64) (rs1_val : BitVec 64) :  MUL_pure64_fff  (rs2_val) (rs1_val )
-          = MUL_pure64_fff_bv  (rs2_val) (rs1_val ) :=
-    by
+theorem MUL_pure64_fff_eq_MUL_pure64_fff_bv (rs2_val : BitVec 64) (rs1_val : BitVec 64) :  MUL_pure64_fff  (rs2_val) (rs1_val)
+    = MUL_pure64_fff_bv  (rs2_val) (rs1_val ) := by
     simp only  [MUL_pure64_fff,  MUL_pure64_fff_bv]
     apply BitVec.eq_of_toNat_eq
     simp only [HMul.hMul, Mul.mul]
@@ -528,7 +504,7 @@ def  MUL_pure64_fft (rs2_val : BitVec 64) (rs1_val : BitVec 64) : BitVec 64 :=
     (BitVec.extractLsb' 0 128
       (BitVec.ofInt 129 (Int.ofNat (Int.mul (Int.ofNat rs1_val.toNat)  (rs2_val.toInt)).toNat)))
 
--- this case is never used
+-- no risc-v instruction maps to this multiplication with the combination of flags ftf.
 def MUL_pure64_ftf (rs2_val : BitVec 64) (rs1_val : BitVec 64)  : BitVec 64 :=
   BitVec.extractLsb 63 0 (BitVec.extractLsb' 0 128 (BitVec.ofInt 129 (rs1_val.toInt * rs2_val.toNat)))
 
@@ -540,7 +516,6 @@ def MUL_pure64_tff (rs2_val : BitVec 64) (rs1_val : BitVec 64) : BitVec 64 :=
 
 def MUL_pure64_tff_bv  (rs2_val : BitVec 64) (rs1_val : BitVec 64) : BitVec 64 :=
    BitVec.extractLsb 127 64 (BitVec.extractLsb' 0 128 ((BitVec.zeroExtend 128 rs1_val)  * (BitVec.zeroExtend 128 rs2_val)))
-
 
 theorem MUL_pure64_tff_eq_MUL_pure64_tff_bv  (rs2_val : BitVec 64) (rs1_val : BitVec 64)  :
   MUL_pure64_tff (rs2_val) (rs1_val) = MUL_pure64_tff_bv (rs2_val) (rs1_val) := by
@@ -566,8 +541,7 @@ theorem MUL_pure64_tff_eq_MUL_pure64_tff_bv  (rs2_val : BitVec 64) (rs1_val : Bi
       by
       rw [cc]
       have := Nat.mul_lt_mul'' (a := rs1_val.toNat) (b := rs2_val.toNat) (c := 2 ^ 64) (d := 2 ^ 64) aa bb
-      omega
-       )]
+      omega )]
     have := @Nat.mul_lt_mul'' _ _ _ _ aa bb
     simp only [Nat.reducePow, Nat.reduceMul] at this
     omega
@@ -584,7 +558,7 @@ def MUL_pure64_ttf (rs2_val : BitVec 64) (rs1_val : BitVec 64) : BitVec 64 :=
   BitVec.extractLsb 127 64 (BitVec.extractLsb' 0 128 (BitVec.ofInt 129 (rs1_val.toInt * rs2_val.toNat)))
 
 def MUL_pure64_ttf_bv (rs2_val : BitVec 64) (rs1_val : BitVec 64) : BitVec 64 :=
-  BitVec.extractLsb 127 64 (((BitVec.signExtend 129 rs1_val )* (BitVec.zeroExtend 129 rs2_val )))
+  BitVec.extractLsb 127 64 (((BitVec.signExtend 129 rs1_val ) * (BitVec.zeroExtend 129 rs2_val )))
 
 theorem MUL_pure64_ttf_eq_MUL_pure64_ttf_bv (rs2_val : BitVec 64) (rs1_val : BitVec 64) :
    MUL_pure64_ttf (rs2_val) (rs1_val) = MUL_pure64_ttf_bv (rs2_val) (rs1_val) := by
@@ -611,7 +585,7 @@ def MUL_pure64_ftt (rs2_val : BitVec 64) (rs1_val : BitVec 64) : BitVec 64 :=
 def MUL_pure64_ftt_bv  (rs2_val : BitVec 64) (rs1_val : BitVec 64) : BitVec 64 :=
   rs2_val * rs1_val
 
-theorem mul_eq_mul_ftt_pretty (rs2_val : BitVec 64) (rs1_val : BitVec 64) :  MUL_pure64_ftt  (rs2_val) (rs1_val )
+theorem MUL_pure64_ftt_eq_MUL_pure64_ftt_bv (rs2_val : BitVec 64) (rs1_val : BitVec 64) :  MUL_pure64_ftt  (rs2_val) (rs1_val )
      = MUL_pure64_ftt_bv  (rs2_val) (rs1_val ) :=
   by
   unfold  MUL_pure64_ftt  MUL_pure64_ftt_bv
@@ -633,8 +607,6 @@ theorem mul_eq_mul_ftt_pretty (rs2_val : BitVec 64) (rs1_val : BitVec 64) :  MUL
 def MUL_pure64_ttt (rs2_val : BitVec 64) (rs1_val : BitVec 64) : BitVec 64 :=
   BitVec.extractLsb 127 64 (BitVec.extractLsb' 0 128 (BitVec.ofInt 129 (rs1_val.toInt * rs2_val.toInt)))
 
--- need to first signed extend it and then compute mul and then shorten it :: to do
--- check my rewrite
 def MUL_pure64_ttt_bv  (rs2_val : BitVec 64) (rs1_val : BitVec 64) : BitVec 64 :=
  BitVec.extractLsb 127 64 ((BitVec.signExtend 129 rs1_val) *  (BitVec.signExtend 129 rs2_val))
 
@@ -652,6 +624,7 @@ theorem MUL_pure64_ttt_eq_MUL_pure64_ttt_bv (rs2_val : BitVec 64) (rs1_val : Bit
     simp only [BitVec.ofInt_toInt, extractLsb'_eq_setWidth]
     rw [extractLsb_setWidth_of_lt (hi := 127) (lo := 64) (v := 128) (x := BitVec.signExtend 129 rs1_val * BitVec.signExtend 129 rs2_val) (by omega)]
     simp
+
 -- to do
 def DIVW_pure64_signed (rs2_val : BitVec 64) (rs1_val : BitVec 64) : BitVec 64 :=
   BitVec.signExtend 64
@@ -686,15 +659,7 @@ def DIV_pure64_signed_bv (rs2_val : BitVec 64) (rs1_val : BitVec 64) : BitVec 64
   else
     rs1_val.sdiv rs2_val
 
--- show Type        from Value ~= (Value : Type)
--- show Proposition from Proof ~= (Value : Type)
-
-theorem neg_ofNat_eq_ofInt_neg {w : Nat} (x : Nat) :
-    - BitVec.ofNat w x = BitVec.ofInt w (- x) := by
-  apply BitVec.eq_of_toInt_eq
-  simp [BitVec.toInt_neg, BitVec.toInt_ofNat]
-
-theorem DIV_pure64_signed_eq_DIV_pure64_signed_bv  (rs2_val : BitVec 64) (rs1_val : BitVec 64)  :
+theorem DIV_pure64_signed_eq_DIV_pure64_signed_bv (rs2_val : BitVec 64) (rs1_val : BitVec 64)  :
   DIV_pure64_signed (rs2_val) (rs1_val ) = DIV_pure64_signed_bv (rs2_val) (rs1_val ) := by
     unfold DIV_pure64_signed DIV_pure64_signed_bv
     rw [extractLsb'_ofInt_eq_ofInt (h:= by simp)]
@@ -783,15 +748,14 @@ def ITYPE_pure64_RISCV_ORI (imm : BitVec 12) (rs1_val : BitVec 64) : BitVec 64 :
       let immext : BitVec 64 := (BitVec.signExtend 64 imm) ;
       BitVec.or rs1_val immext
 
-
-def  ITYPE_pure64_RISCV_XORI (imm : (BitVec 12)) (rs1_val : (BitVec 64)) : BitVec 64 :=
+def  ITYPE_pure64_RISCV_XORI (imm : BitVec 12) (rs1_val : BitVec 64) : BitVec 64 :=
       let immext : BitVec 64 := (BitVec.signExtend 64 imm) ;
       BitVec.xor rs1_val immext
 
-def ZICOND_RTYPE_pure64_RISCV_CZERO_EQZ (rs2_val : (BitVec 64)) (rs1_val : (BitVec 64)) :=
+def ZICOND_RTYPE_pure64_RISCV_CZERO_EQZ (rs2_val : BitVec 64) (rs1_val : BitVec 64) :=
       (if rs2_val = BitVec.zero 64 then BitVec.zero 64 else rs1_val)
 
-def ZICOND_RTYPE_pure64_RISCV_RISCV_CZERO_NEZ (rs2_val : (BitVec 64)) (rs1_val : (BitVec 64)) :=
+def ZICOND_RTYPE_pure64_RISCV_RISCV_CZERO_NEZ (rs2_val : BitVec 64) (rs1_val : BitVec 64) :=
    (if rs2_val = BitVec.zero 64 then rs1_val else BitVec.zero 64)
 
 def ZBS_RTYPE_pure64_RISCV_BCLR (rs2_val : BitVec 64) (rs1_val : BitVec 64) :=
@@ -907,7 +871,7 @@ def ZBS_IOP_pure64_RISCV_BSETI (shamt : BitVec 6) (rs1_val : BitVec 64) :=
   BitVec.or rs1_val (BitVec.shiftLeft (BitVec.zeroExtend 64 1#1) shamt.toNat)
 
 def ZBS_IOP_pure64_RISCV_BSETI_bv (shamt : BitVec 6) (rs1_val : BitVec 64) :=
-  BitVec.or rs1_val ( (BitVec.zeroExtend 64 1#1) <<< shamt)
+  BitVec.or rs1_val ((BitVec.zeroExtend 64 1#1) <<< shamt)
 
 theorem ZBS_IOP_pure64_RISCV_BSETI_eq_ZBS_IOP_pure64_RISCV_BSETI_bv (shamt : BitVec 6) (rs1_val : BitVec 64) :
   ZBS_IOP_pure64_RISCV_BSETI (shamt) (rs1_val) =   ZBS_IOP_pure64_RISCV_BSETI_bv (shamt) (rs1_val) :=
